Tidy up coq files

coq/as_prover.v
@@ -5,23 +5,19 @@ Definition t := As_prover.t.
 
 Section Instances.
 
-  Polymorphic Variables f v s : Type.
+  Polymorphic Variables (f v s : Type).
 
-  Global Polymorphic Instance as_prover_map f v s : Map (t f v s) := {
-    map := fun A B t f tbl s =>
-      let (s', x) := t tbl s in
-      (s', f x)
-  }.
+  Global Polymorphic
+Instance as_prover_map  f v s: (Map (t f v s)) := {
+ map :=fun A B t f tbl s => let (s', x) := t tbl s in (s', f x)}.
 
-  Global Polymorphic Instance as_prover_bind f v s : Bind (t f v s) := {
-    bind := fun A B t f tbl s =>
-      let (s', x) := t tbl s in
-      f x tbl s'
-  }.
+  Global Polymorphic
+Instance as_prover_bind  f v s: (Bind (t f v s)) := {
+ bind :=fun A B t f tbl s => let (s', x) := t tbl s in f x tbl s'}.
 
-  Global Polymorphic Instance as_prover_ret f v s : Return (t f v s) := {
-    ret := fun A x _ s => (s, x)
-  }.
+  Global Polymorphic
+Instance as_prover_ret  f v s: (Return (t f v s)) := {
+ ret :=fun A x _ s => (s, x)}.
 
 End Instances.
 
@@ -48,24 +44,21 @@ Module T.
     Context {F V S : Type}.
 
     Definition run {S A : Type} : t F V S A -> (V -> F) -> S -> S * A :=
-      fun t tbl s => t tbl s.
+  fun t tbl s => t tbl s.
 
-    Definition get_state {S : Type} : t F V S S :=
-      fun _tbl s => (s, s).
+    Definition get_state {S : Type} : t F V S S := fun _tbl s => (s, s).
 
     Definition set_state {S : Type} : S -> t F V S unit :=
-      fun s _tbl _ => (s, tt).
+  fun s _tbl _ => (s, tt).
 
     Definition modify_state {S : Type} : (S -> S) -> t F V S unit :=
-      fun f _tbl s => (f s, tt).
+  fun f _tbl s => (f s, tt).
 
-    Definition read_var (v : V) : t F V S F :=
-      fun tbl s => (s, tbl v).
+    Definition read_var (v : V) : t F V S F := fun tbl s => (s, tbl v).
 
     Definition read {f v sys s var value : Type} {request : Type -> Type}
-      (typ : Snarky.types.Typ.t f v sys request var value) (var : var)
-    : t f v s value :=
-      fun tbl s => (s, typ_monads.Read.run (Typ.read typ var) tbl).
+  (typ : Typ.t f v sys request var value) (var : var) : t f v s value :=
+  fun tbl s => (s, typ_monads.Read.run (Typ.read typ var) tbl).
 
   End T.
     
