coq/checked.v
@@ -331,3 +331,5 @@ Module Run.
     ; stack := []
     |} in
     run_aux rstate t.
+End Run_aux.
+End Run.
