coq/field.v
@@ -1,71 +1,69 @@
 Section Field.
 
-  Variable F : Type.
+  Variable (F : Type).
 
   (** Left general in case we want to use nat and Z, etc. *)
-  Class Of_int (A : Type) := { of_int : A -> F }.
+  Class Of_int (A : Type) :={of_int : A -> F}.
 
-  Class One := { one : F }.
+  Class One :={one : F}.
 
-  Class Zero := { zero : F }.
+  Class Zero :={zero : F}.
 
-  Class Add := { add : F -> F -> F }.
+  Class Add :={add : F -> F -> F}.
 
-  Class Sub := { sub : F -> F -> F }.
+  Class Sub :={sub : F -> F -> F}.
 
-  Class Mul := { mul : F -> F -> F }.
+  Class Mul :={mul : F -> F -> F}.
 
-  Class Inv := { inv : F -> F }.
+  Class Inv :={inv : F -> F}.
 
-  Class Square := { square : F -> F }.
+  Class Square :={square : F -> F}.
 
-  Class Sqrt := { sqrt : F -> F }.
+  Class Sqrt :={sqrt : F -> F}.
 
-  Class Is_square := { is_square : F -> bool }.
+  Class Is_square :={is_square : F -> bool}.
 
-  Class Equal := { equal : F -> F -> bool }.
+  Class Equal :={equal : F -> F -> bool}.
 
-  Class Size_in_bits (F : Type) (A : Type) := { size_in_bits : A }.
+  Class Size_in_bits (F : Type) (A : Type) :={size_in_bits : A}.
 
   Definition negate `{Sub} `{Zero} x := sub zero x.
 
 End Field.
 
 Module Class.
-  Class Field (F A : Type) := {
-    field_of_int :> Of_int F A;
-    field_one :> One F;
-    field_zero :> Zero F;
-    field_add :> Add F;
-    field_sub :> Sub F;
-    field_mul :> Mul F;
-    field_inv :> Inv F;
-    field_square :> Square F;
-    field_sqrt :> Sqrt F;
-    field_is_square :> Is_square F;
-    field_equal :> Equal F;
-    field_size_in_bits :> Size_in_bits F A
-  }.
+  Class Field (F A : Type) :={field_of_int :> Of_int F A;
+                            field_one :> One F;
+                            field_zero :> Zero F;
+                            field_add :> Add F;
+                            field_sub :> Sub F;
+                            field_mul :> Mul F;
+                            field_inv :> Inv F;
+                            field_square :> Square F;
+                            field_sqrt :> Sqrt F;
+                            field_is_square :> Is_square F;
+                            field_equal :> Equal F;
+                            field_size_in_bits :> Size_in_bits F A}.
 End Class.
 Include Class.
 
-Arguments of_int {F A Of_int} _.
-Arguments one {F One}.
-Arguments zero {F Zero}.
-Arguments add {F Add} _ _.
-Arguments sub {F Sub} _ _.
-Arguments mul {F Mul} _ _.
-Arguments inv {F Inv} _.
-Arguments square {F Square} _.
-Arguments sqrt {F Sqrt} _.
-Arguments is_square {F Is_square} _.
-Arguments equal {F Equal} _ _.
-Arguments size_in_bits {F A Size_in_bits}.
-Arguments negate {F Sub Zero} _ : rename.
+Arguments of_int {F} {A} {Of_int} _.
+Arguments one {F} {One}.
+Arguments zero {F} {Zero}.
+Arguments add {F} {Add} _ _.
+Arguments sub {F} {Sub} _ _.
+Arguments mul {F} {Mul} _ _.
+Arguments inv {F} {Inv} _.
+Arguments square {F} {Square} _.
+Arguments sqrt {F} {Sqrt} _.
+Arguments is_square {F} {Is_square} _.
+Arguments equal {F} {Equal} _ _.
+Arguments size_in_bits {F} {A} {Size_in_bits}.
+Arguments negate {F} {Sub} {Zero} _ : rename.
 
 Module FieldNotation.
 
-  Infix "+" := plus.
+  Infix "+" := Nat.add.
   Infix "*" := mul.
   Infix "-" := sub.
   Infix "/" := (fun x y => mul x (inv y)).
